Refactor eutt_loop with sutt

theories/Eq/SimUpToTaus.v
@@ -29,6 +29,21 @@ Inductive suttF (eutt : itree E R1 -> itree E R2 -> Prop)
 .
 Hint Constructors suttF.
 
+Lemma suttF_unpack eutt ot1 ot2 :
+  suttF eutt ot1 ot2 <->
+  forall ot1', unalltausF ot1 ot1' ->
+  exists ot2', unalltausF ot2 ot2' /\ eq_notauF RR eutt ot1' ot2'.
+Proof.
+  split.
+  - intros [] ot1' H1.
+    edestruct FIN; eauto.
+  - intros. constructor.
+    + intros []; auto. edestruct H as [? []]; eauto.
+    + intros; edestruct H as [y []]; eauto.
+      replace ot2' with y; auto.
+      eapply unalltaus_injective; eauto.
+Qed.
+
 Definition sutt_ (eutt : itree E R1 -> itree E R2 -> Prop)
            (t1 : itree E R1) (t2 : itree E R2) : Prop :=
   suttF eutt (observe t1) (observe t2).
@@ -54,6 +69,23 @@ Hint Constructors suttF.
 Hint Unfold sutt_.
 Hint Resolve monotone_sutt_ : paco.
 
+Lemma monotone_eq_notauF_RR {E R1 R2} (RR1 RR2 : R1 -> R2 -> Prop)
+      {I J} (r : I -> J -> Prop) :
+  (forall r1 r2, RR1 r1 r2 -> RR2 r1 r2) ->
+  forall t1 t2, eq_notauF RR1 r t1 t2 -> @eq_notauF E _ _ RR2 _ _ r t1 t2.
+Proof. intros ? ? ? []; auto. Qed.
+
+Lemma monotone_sutt_RR {E R1 R2} (RR1 RR2 : R1 -> R2 -> Prop) r :
+  (forall r1 r2, RR1 r1 r2 -> RR2 r1 r2) ->
+  forall t1 t2, sutt_ RR1 r t1 t2 -> @sutt_ E _ _ RR2 r t1 t2.
+Proof.
+  intros. induction H0.
+  constructor; auto.
+  intros.
+  edestruct EQV; eauto;
+    eapply monotone_eq_notauF_RR; eauto.
+Qed.
+
 Theorem sutt_eutt {E R1 R2} (RR : R1 -> R2 -> Prop) :
   forall (t1 : itree E R1) (t2 : itree E R2),
     sutt RR t1 t2 -> sutt (flip RR) t2 t1 -> eutt RR t1 t2.
@@ -72,4 +104,111 @@ Proof.
     + apply eq_notauF_flip.
       eapply monotone_eq_notauF; auto using EQV2.
       intros; pclearbot; auto.
+Qed.
+
+Theorem eutt_sutt {E R1 R2} (RR : R1 -> R2 -> Prop) :
+  forall (t1 : itree E R1) (t2 : itree E R2),
+    eutt RR t1 t2 -> sutt RR t1 t2.
+Proof.
+  pcofix self; intros t1 t2 H1.
+  punfold H1.
+  destruct H1 as [FIN1 EQV1].
+  pfold; constructor.
+  - apply FIN1.
+  - intros.
+    eapply monotone_eq_notauF; eauto.
+    intros; pclearbot; auto.
+Qed.
+
+Inductive suttF' {E R} (sutt: relation (itree E R)) :
+  relation (itree' E R) :=
+| suttF'_notau ot1 ot2 ot2' :
+    unalltausF ot2 ot2' ->
+    eq_notauF eq sutt ot1 ot2' ->
+    suttF' sutt ot1 ot2
+| suttF'_tau_left t1 ot2
+      (EQTAUS: suttF' sutt (observe t1) ot2):
+    suttF' sutt (TauF t1) ot2
+.
+Hint Constructors suttF'.
+
+Theorem suttF_suttF' {E R} (sutt : relation (itree E R)) :
+  forall ot1 ot2,
+    suttF eq sutt ot1 ot2 <-> suttF' sutt ot1 ot2.
+Proof.
+Admitted.
+
+Inductive suttF1 {E R} (sutt: itree' E R -> itree' E R -> Prop) :
+  itree' E R -> itree' E R -> Prop :=
+| suttF1_ret r : suttF1 sutt (RetF r) (RetF r)
+| suttF1_vis u (e : E u) k1 k2
+      (SUTTK: forall x, sutt (observe (k1 x)) (observe (k2 x))):
+    suttF1 sutt (VisF e k1) (VisF e k2)
+| suttF1_tau_right ot1 t2
+      (EQTAUS: suttF1 sutt ot1 (observe t2)):
+    suttF1 sutt ot1 (TauF t2)
+| suttF1_tau_left t1 ot2
+      (EQTAUS: sutt (observe t1) ot2):
+    suttF1 sutt (TauF t1) ot2
+.
+Hint Constructors suttF1.
+
+Definition sutt1 {E R} (t1 t2 : itree E R) :=
+  paco2 (@suttF1 E R) bot2 (observe t1) (observe t2).
+Hint Unfold sutt1.
+
+Lemma reflexive_suttF1 {E R} sutt (r1:Reflexive sutt) : Reflexive (@suttF1 E R sutt).
+Proof.
+  unfold Reflexive. intros x.
+  destruct x; eauto.
+Qed.
+
+Lemma monotone_suttF1 {E R} : monotone2 (@suttF1 E R).
+Proof. repeat red; intros. induction IN; eauto. Qed.
+Hint Resolve monotone_suttF1 : paco.
+
+Lemma sutt_is_sutt1 {E R} (t1 t2: itree E R) :
+  sutt eq t1 t2 <-> sutt1 t1 t2.
+Proof.
+  split; revert t1 t2; pcofix self; intros t1 t2 SUTT.
+  - punfold SUTT. pfold.
+    apply suttF_suttF' in SUTT.
+    induction SUTT; auto.
+    destruct H as [Huntaus Hnotau].
+    induction Huntaus.
+    + inversion H0; subst; constructor.
+      pclearbot. right; apply self; red; auto.
+    + subst; auto.
+  - punfold SUTT. pfold.
+    red.
+    induction SUTT.
+    + constructor; eauto. intros.
+      apply unalltausF_ret in UNTAUS1.
+      apply unalltausF_ret in UNTAUS2.
+      subst; auto.
+    + constructor; eauto 7. intros.
+      apply unalltausF_vis in UNTAUS1.
+      apply unalltausF_vis in UNTAUS2.
+      pclearbot; subst; auto.
+      constructor. right; auto.
+    + destruct IHSUTT; constructor; intros.
+      * apply finite_taus_tau; auto.
+      * apply EQV. auto. eapply unalltaus_tau; eauto.
+    + pclearbot; punfold EQTAUS.
+      eapply suttF_unpack.
+      intros t0' Hunalltaus.
+      eapply unalltaus_tau in Hunalltaus; eauto.
+      destruct Hunalltaus as [Huntaus Hnotau].
+      revert ot2 EQTAUS.
+      induction Huntaus; intros.
+      * induction EQTAUS;
+          contradiction + eauto 6.
+        { pclearbot. econstructor. repeat (constructor; auto). }
+        { destruct IHEQTAUS as [ot2' []]; auto.
+          eexists; split; eauto using unalltaus_tau'. }
+      * induction EQTAUS;
+          discriminate + eauto 6.
+        { destruct IHEQTAUS as [? []]; auto.
+          eexists; eauto using unalltaus_tau'. }
+        { pclearbot. inv OBS. punfold EQTAUS; auto. }
 Qed.
